\documentclass{article}
\usepackage{amsmath}
\usepackage{amssymb}
\usepackage[margin=2cm]{geometry}
\usepackage[english]{babel}
\author{Kevin Michael Frick}
\title{OTDM - Optimality conditions homework}
\begin{document}
\maketitle
Problem statement:

\begin{equation*}
\begin{cases}
\min &(x_1 - 3)^2 + (x_2 - 2)^2  \\
\textsc{s.t.} & x_1^2 + x_2^2 \leq 1
\end{cases}
\end{equation*}

We first calculate the Lagrangian. In this case, the single inequality constraint is real-valued, so $\mu$ is a scalar.

$$L(x, \mu) = (x_1 - 3)^2 + (x_2 - 2)^2 + \mu(x_1^2 + x_2^2 - 1)$$

The gradient of the Lagrangian w.r.t. $\mathbf{x}$ is

$$\nabla_x L = (2 x_1 + 2\mu x_1 - 6, 2x_2 + 2 \mu x_2 - 4)$$ 

and its Hessian is

$$\nabla^2_{xx} L = \begin{pmatrix} 2 + 2 \mu & 0 \\ 0 & 2 + 2 \mu\end{pmatrix}$$

whose eigevalues are

$$\lambda(\nabla^2_{xx} L) = \{2 + 2 \mu\}$$

Imposing the KKT sufficient first- and second-order conditions we get

\begin{equation*}
\begin{cases}
(1 + \mu) x_1 - 3 = 0 \\
(1 + \mu) x_2 - 2 = 0 \\
x_1^2 + x_2^2 \leq 1 \\
\mu(x_1^2 + x_2^2 - 1) = 0 \\
\mu \geq 0 \\
2 + 2\mu > 0
\end{cases}
\end{equation*}

The last equation evaluates to $\mu > -1$ which is redundant. 

Solving the first and second equation leads to 
\begin{equation*}
\begin{cases}
x_1 = \frac{3}{1 + \mu} \\
x_2 = \frac{2}{1 + \mu} 
\end{cases}
\end{equation*}

Which substituted into the complementary slackness condition gives

$$
\mu (\frac{9}{(1 + \mu)^2} + \frac{4}{(1 + \mu)^2} - 1) = 0
$$

If we assume $\mu = 0$ we get $x_1 = 3, x_1 = 2$ but then $x_1^2 + x_2^2 > 1$, so $\mu \neq 0$. 
Therefore we can solve complementary slackness for $\mu$ and get

$$13 = (1 + \mu)^2 \iff 1 + \mu = \pm \sqrt{13}$$

but $\mu > 0$, so

$$\mu = + \sqrt{13} - 1$$

which backsubstituted gives

\begin{equation*}
\begin{cases}
x_1 = \frac{3\sqrt{13}}{13} \\
x_2 = \frac{2\sqrt{13}}{13} 
\end{cases}
\end{equation*}

which verify $x_1^2 + x_2^2 \leq 1$ (in particular, $x_1^2 + x_2^2 = 1$, so the point is on the circumference). 

Therefore the solution of the problem is 

$$
\mathbf{x} = \frac{\sqrt{13}}{13} (3, 2)
$$

This is, clearly, not a global minimum for the unconstrained $f(x_1, x_2) = (x_1 - 3)^2 + (x_2 - 2)^2$, as the global minimum is $(3, 2)$ where $f(3, 2) = 0$. 
However, given the constraint, there is only one minimum which is the point we just found. 
Since the point lies on the circumference, if the constraint had been an equality constraint the solution would have been the same. 

\end{document}
